**HW: p.27-28 #3, 11, 17(b);p.38 #7**

**#3** 
a:0.15 b:0.9 c:1.5 d:0.09

**#11**
* ***a:**
	$f(x)=\frac{cox-\frac{sinx}{x}}{1-\frac{sinx}{x}}$
	use taylor expansion, then:
	$sinx=x-\frac{x^3}{6}+o(x^3)$
	$cosx=1-\frac{x^2}{2}+o(x^2)$
	so that
	$f(x)=\frac{-\frac{x^2}{3}+o(x^2)}{\frac{x^2}{6}+o(x^2)}$
	$f(0)=-2$
* **b:**
	$f(0.1)=\frac{0.1\times0.9950-0.09983}{0.1-0.09983}$
	$=\frac{9.950\times10^{-2}-9.983\times10^{-2}}{10.00\times10^{-2}-9.98\times10^{-2}}$
	=$\frac{-3.300\times10^{-4}}{2\times10^{-4}}$
	=$-1.650$
* **c:**
	$sinx=x-\frac{x^3}{6}+\frac{x^5}{120}$
	$cosx=1-\frac{x^2}{2}+\frac{x^4}{24}$
	$sin(0.1)=0.1-\frac{10^{-3}}{6}+\frac{10^{-5}}{120}$=$0.1002$
	$cos(0.1)=1-\frac{10^{-2}}{2}+\frac{10^{-4}}{120}$=0.9950
	$f(0.1)=\frac{0.1*0.9950-0.1002}{0.1-0.1002}$
	$=\frac{0.0995-0.1002}{0.0002}$
	$=-3.5$
* d:
	part b: $E_b=|\frac{f(0.1)+1.650}{f(0.1)}|$ = 0.1746
	part c: $E_c=|\frac{f(0.1)+3.5}{(0.1)}|$=0.7509

**#7**
a: $h^2$  b: h  c: $h^2$  d: h